src/Memory.v
@@ -13,21 +13,64 @@ Definition Size := N.
 Definition Word := Ascii.ascii.
 Definition Zero := Ascii.zero.
 
-Definition plusPtr `(ptr : Ptr A) (n : Size) := (ptr + n)%N.
-Definition minusPtr `(ptr : Ptr A) (n : Size) := (ptr - n)%N.
+Definition eqPtr {A} (x y : Ptr A) := x = y.
+Hint Unfold eqPtr.
+Definition neqPtr {A} (x y : Ptr A) := x <> y.
+Hint Unfold neqPtr.
+Definition eqbPtr {A} (x y : Ptr A) := N.eqb x y.
+Hint Unfold eqbPtr.
+Definition eqdecPtr {A} (x y : Ptr A) := N.eq_dec x y.
+Hint Unfold eqdecPtr.
+
+Definition ltPtr {A} (ptr1 ptr2 : Ptr A) : Prop := N.lt ptr1 ptr2.
+Hint Unfold ltPtr.
+Definition lePtr {A} (ptr1 ptr2 : Ptr A) : Prop := N.le ptr1 ptr2.
+Hint Unfold lePtr.
+Definition gtPtr {A} (ptr1 ptr2 : Ptr A) : Prop := N.gt ptr1 ptr2.
+Hint Unfold gtPtr.
+Definition gePtr {A} (ptr1 ptr2 : Ptr A) : Prop := N.ge ptr1 ptr2.
+Hint Unfold gePtr.
+
+Definition ltbPtr {A} (ptr1 ptr2 : Ptr A) : bool := N.ltb ptr1 ptr2.
+Hint Unfold ltbPtr.
+Definition lebPtr {A} (ptr1 ptr2 : Ptr A) : bool := N.leb ptr1 ptr2.
+Hint Unfold lebPtr.
+
+Delimit Scope Ptr_scope with Ptr.
+Bind Scope Ptr_scope with Ptr.
+
+Infix "<=" := lePtr : Ptr_scope.
+Infix "<"  := ltPtr : Ptr_scope.
+Infix ">=" := gePtr : Ptr_scope.
+Infix ">"  := gtPtr : Ptr_scope.
+
+Notation "x <= y <= z" := (x <= y /\ y <= z)%Ptr : Ptr_scope.
+Notation "x <= y <  z" := (x <= y /\ y <  z)%Ptr : Ptr_scope.
+Notation "x <  y <  z" := (x <  y /\ y <  z)%Ptr : Ptr_scope.
+Notation "x <  y <= z" := (x <  y /\ y <= z)%Ptr : Ptr_scope.
+
+Infix "=?"  := eqbPtr (at level 70, no associativity) : Ptr_scope.
+Infix "<=?" := lebPtr (at level 70, no associativity) : Ptr_scope.
+Infix "<?"  := ltbPtr (at level 70, no associativity) : Ptr_scope.
+
+Definition plusPtr  `(ptr : Ptr A) (n : Size) := (ptr + n)%N.
+Hint Unfold plusPtr.
+Definition minusPtr {A} (ptr1 ptr2 : Ptr A) := (ptr1 - ptr2)%N.
+Hint Unfold minusPtr.
 
 Module Ptr_as_OT <: UsualOrderedType.
   Definition t:=Ptr Word.
-  Definition eq:=@eq (Ptr Word).
-  Definition eq_refl := @eq_refl t.
-  Definition eq_sym := @eq_sym t.
+  Definition eq:=eqPtr (A:=Word).
+
+  Definition eq_refl  := @eq_refl t.
+  Definition eq_sym   := @eq_sym t.
   Definition eq_trans := @eq_trans t.
 
-  Definition lt := N.lt.
+  Definition lt := ltPtr (A:=Word).
   Definition lt_trans := N.lt_trans.
   Definition lt_not_eq := N.lt_neq.
 
-  Definition compare x y : Compare lt eq x y.
+  Definition compare x y : Compare (ltPtr (A:=Word)) (eqPtr (A:=Word)) x y.
   Proof.
   case_eq (x ?= y)%N; intro.
   - apply EQ. now apply N.compare_eq.
@@ -35,7 +78,7 @@ Module Ptr_as_OT <: UsualOrderedType.
   - apply GT. now apply N.gt_lt.
   Defined.
 
-  Definition eq_dec := N.eq_dec.
+  Definition eq_dec := eqdecPtr (A:=Word).
 End Ptr_as_OT.
 
 Module Ptr_as_DT <: UsualDecidableType := Ptr_as_OT.
@@ -62,33 +105,16 @@ Corollary plusPtr_succ : forall A (addr : Ptr A) n,
   plusPtr (A:=A) (plusPtr addr n) 1 = plusPtr addr (N.succ n).
 Proof. intros; nomega. Qed.
 
-Corollary plusPtr_sub : forall A (addr : Ptr A) n m,
-  m <= n -> minusPtr (A:=A) (plusPtr addr n) m = plusPtr addr (n - m).
-Proof. intros; symmetry; apply N.add_sub_assoc; nomega. Qed.
-
-Corollary plusPtr_sub_r : forall A (addr : Ptr A) n m,
-  n <= addr -> n <= m
-    -> plusPtr (A:=A) (minusPtr addr n) m = plusPtr addr (m - n).
-Proof. intros; nomega. Qed.
-
 Corollary plusPtr_comm : forall A (addr : Ptr A) n m,
   plusPtr (A:=A) (plusPtr addr n) m = plusPtr (A:=A) (plusPtr addr m) n.
 Proof. intros; nomega. Qed.
 
-Corollary minusPtr_add : forall A (addr : Ptr A) n m,
-  minusPtr (A:=A) (minusPtr addr n) m = minusPtr addr (n + m).
+Corollary minusPtr_plusPtr_plusPtr : forall A (addr : Ptr A) n m,
+  minusPtr (A:=A) (plusPtr addr n) (plusPtr addr m) = n - m.
 Proof. intros; nomega. Qed.
 
-Corollary minusPtr_zero : forall A (addr : Ptr A),
-  minusPtr addr 0 = addr.
-Proof. intros; nomega. Qed.
-
-Corollary minusPtr_succ : forall A (addr : Ptr A) n,
-  n <= addr -> minusPtr (A:=A) (minusPtr addr 1) n = minusPtr addr (N.succ n).
-Proof. intros; nomega. Qed.
-
-Corollary minusPtr_sub : forall A (addr : Ptr A) n m,
-  m <= n -> minusPtr (A:=A) (plusPtr addr m) n = minusPtr addr (n - m).
+Corollary minusPtr_plusPtr : forall A (addr : Ptr A) n,
+  minusPtr (A:=A) (plusPtr addr n) addr = n.
 Proof. intros; nomega. Qed.
 
 Hint Rewrite N.add_0_r : ptr.
@@ -101,12 +127,9 @@ Hint Rewrite succ_sub_one : ptr.
 Hint Rewrite succ_one_sub : ptr.
 Hint Rewrite plusPtr_zero : ptr.
 Hint Rewrite plusPtr_add : ptr.
-Hint Rewrite plusPtr_sub : ptr.
 Hint Rewrite plusPtr_succ : ptr.
-Hint Rewrite minusPtr_zero : ptr.
-Hint Rewrite minusPtr_add : ptr.
-Hint Rewrite minusPtr_sub : ptr.
-Hint Rewrite minusPtr_succ : ptr.
+Hint Rewrite minusPtr_plusPtr_plusPtr : ptr.
+Hint Rewrite minusPtr_plusPtr : ptr.
 
 Ltac rewrite_ptr :=
   repeat (
